Connect/Extra.v
@@ -1,0 +1,34 @@
+Require Import Accessors.Spec.
+Require Import Bottom.Spec.
+Require Import CommonDeps.
+Require Import DataTypes.
+Require Import GlobalDefs.
+Require Import LayerSem.Libs.Zutils.div_mod_to_equations.
+
+Local Open Scope string_scope.
+Local Open Scope Z_scope.
+Local Opaque Z.add Z.mul Z.div Z.sub Z.land Z.lor Z.lxor Z.shiftl Z.shiftr Z.quot Z.rem.
+
+Require Import LayerSem.Libs.Zutils.BitOps.
+Require Import LayerSem.Libs.Zutils.hardcode_rewrite.
+
+Definition lshl (n digit : Z) : Z :=
+  n * (2 ^ digit).
+
+Definition lshr (n digit : Z) : Z :=
+  n / (2 ^ digit).
+
+Definition substr (n head tail : Z) : Z :=
+  lshr (n mod (2 ^ (head + 1))) tail.
+
+Definition substr_eq : forall z,
+  is_addr z -> substr z 47 21 = z / 4096 / 512.
+Proof.
+  intros.
+  unfold substr. unfold lshr. unfold is_addr, MAX_ADDR in H.
+  change (2 ^ (47 + 1)) with (1 << 48).
+  assert (0 <= z < 1 << 48) by lia.
+  rewrite (Z.mod_small _ _ H0).
+  rewrite Zdiv_Zdiv; [|lia|lia].
+  reflexivity.
+Qed.
